Nicer proof of mtr_td

theories/mtr_td.v
@@ -55,27 +55,32 @@ Section proof.
 Local Set Default Proof Using "Type*".
 Context `{!heapGS Σ}.
 
-Lemma heap_td_insert_correct (i : Z) (tv : val) (t : tree) :
+Definition mtr_insert_td t k := td_insert k t.
+Definition mtr_down_td t k accl accr := td_insert_go k accl accr t.
+
+Lemma heap_td_insert_correct (k : Z) (tv : val) (t : tree) :
     {{{ is_tree t tv }}}
-    heap_mtr_insert_td (ref #i) (ref tv)
-    {{{ v, RET v; is_tree (td_insert i t) v }}}.
+    heap_mtr_insert_td (ref #k) (ref tv)
+    {{{ v, RET v; is_tree (mtr_insert_td t k) v }}}.
 Proof.
   wp_begin "Ht"; name, root. wp_var left_dummy. wp_var right_dummy.
-  wp_load. wp_var node. wp_var left_hook. wp_var right_hook. wp_while_true "H"
-    (∃ l (x : Z) r lv rv (p : loc) lv' rv',
-            root ↦ #p ∗ p ↦∗ [lv'; #x; rv']
-            ∗ left_dummy ↦ lv ∗ is_tree l lv
-            ∗ right_dummy ↦ rv ∗ is_tree r rv
-            ∗ ⌜td_insert i t = Node l x r⌝)%I
-    (∃ lz' rz' t' (lhv rhv : loc) lhvv rhvv rootv treev,
-            node ↦ treev ∗ is_tree t' treev
-            ∗ root ↦ rootv ∗ name ↦ #i
-            ∗ left_hook ↦ #lhv ∗ lhv ↦ lhvv ∗ is_ctx lz' left_dummy lhv
-            ∗ right_hook ↦ #rhv∗ rhv ↦ rhvv ∗ is_ctx rz' right_dummy rhv
-            ∗ ⌜td_insert i t = td_insert_go i lz' rz' t'⌝)%I.
-  - iDecompose "H". wp_type.
-  - iDecompose "H". rewrite H1. wp_type; unfold array; wp_type.
-  - wp_type.
+  wp_load. wp_var node. wp_var left_hook. wp_var right_hook.
+  wp_while_true "H"
+    (∃ l (x : Z) r left_dummy_v right_dummy_v (p : loc) left_dangling_v right_dangling_v,
+            root ↦ #p ∗ p ↦∗ [left_dangling_v; #x; right_dangling_v]
+            ∗ left_dummy ↦ left_dummy_v ∗ is_tree l left_dummy_v
+            ∗ right_dummy ↦ right_dummy_v ∗ is_tree r right_dummy_v
+            ∗ ⌜mtr_insert_td t k = Node l x r⌝)%I
+    (∃ accl accr t' (left_hole right_hole : loc) left_hole_v right_hole_v root_v node_v,
+            node ↦ node_v ∗ is_tree t' node_v
+            ∗ root ↦ root_v ∗ name ↦ #k
+            ∗ left_hook  ↦ #left_hole  ∗ (left_hole  ↦ left_hole_v)  ∗ is_ctx accl left_dummy  left_hole
+            ∗ right_hook ↦ #right_hole ∗ (right_hole ↦ right_hole_v) ∗ is_ctx accr right_dummy right_hole
+            ∗ ⌜mtr_insert_td t k = mtr_down_td t' k accl accr⌝)%I.
+  - iDecompose "H". iSteps.                               (* The claim follows once the while-loop ends *)
+  - iDecompose "H". rewrite H1.                                     (* Rewrite one functional tail-call *)
+    unfold array. repeat (iSteps; try case_bool_decide).            (* Then the invariant is maintained *)
+  - iSteps.                                             (* The preconditions of the while-loop are true *)
 Qed.
 
 End proof.
